Less unicode

Semantics/Imp/Aexp.lean
@@ -3,90 +3,90 @@ import Semantics.Imp.Lang
 namespace Aexp
 namespace Natural
 
-private inductive big_step: Aexp × State → Int → Prop
-  | valₙ: big_step (val₁ n, _) n
-  | varₙ: big_step (var₁ v, s) (s v)
-  | addₙ (ha₁: big_step (a₁, s) n₁) (ha₂: big_step (a₂, s) n₂):
-    big_step (a₁ + a₂, s) (n₁ + n₂)
-  | subₙ (ha₁: big_step (a₁, s) n₁) (ha₂: big_step (a₂, s) n₂):
-    big_step (a₁ - a₂, s) (n₁ - n₂)
-  | mulₙ (ha₁: big_step (a₁, s) n₁) (ha₂: big_step (a₂, s) n₂):
-    big_step (a₁ * a₂, s) (n₁ * n₂)
+private inductive big_step: Aexp × State -> Int -> Prop
+  | val: big_step (val n, _) n
+  | var: big_step (var v, s) (s v)
+  | add (ha: big_step (a, s) x) (ha': big_step (a', s) y):
+    big_step (a + a', s) (x + y)
+  | sub (ha: big_step (a, s) x) (ha': big_step (a', s) y):
+    big_step (a - a', s) (x - y)
+  | mul (ha: big_step (a, s) x) (ha': big_step (a', s) y):
+    big_step (a * a', s) (x * y)
 
-infix:10 " ==>ₐ " => big_step
+infix:10 " ==> " => big_step
 
 private instance big_step.equiv: Setoid Aexp where
-  r a₁ a₂ := ∀{s n}, ((a₁, s) ==>ₐ n) = ((a₂, s) ==>ₐ n)
+  r a a' := ∀{s n}, ((a, s) ==> n) = ((a', s) ==> n)
   iseqv := {
-    refl := λ _ ↦ rfl
-    symm := (·.symm)
-    trans := (· ▸ ·)
+    refl := fun _ => rfl
+    symm := (Eq.symm .)
+    trans := (. ▸ .)
   }
 
-private example: ((var₁ "x" + 5) + (9 - 7), s₀) ==>ₐ 7 :=
-  big_step.addₙ
-    (big_step.addₙ big_step.varₙ big_step.valₙ)
-    (big_step.subₙ big_step.valₙ big_step.valₙ)
+private example: ((var "x" + 5) + (9 - 7), s0) ==> 7 :=
+  big_step.add
+    (big_step.add big_step.var big_step.val)
+    (big_step.sub big_step.val big_step.val)
 
 end Natural
 
 def reduce (a: Aexp) (s: State): Int :=
   match a with
-  | val₁ n => n
-  | var₁ v => s v
-  | add₁ a₁ a₂ => a₁.reduce s + a₂.reduce s
-  | sub₁ a₁ a₂ => a₁.reduce s - a₂.reduce s
-  | mul₁ a₁ a₂ => a₁.reduce s * a₂.reduce s
+  | val n => n
+  | var v => s v
+  | add a a' => reduce a s + reduce a' s
+  | sub a a' => reduce a s - reduce a' s
+  | mul a a' => reduce a s * reduce a' s
 
-instance: CoeFun Aexp (λ _ ↦ State → Int) := ⟨reduce⟩
+instance: CoeFun Aexp (fun _ => State -> Int) := CoeFun.mk reduce
 
 instance reduce.equiv: Setoid Aexp where
-  r a₁ a₂ := ∀{s}, a₁ s = a₂ s
+  r a a' := ∀{s}, a s = a' s
   iseqv := {
-    refl := λ _ ↦ rfl
-    symm := λ h ↦ h.symm
-    trans := λ h₁ h₂ ↦ h₁ ▸ h₂
+    refl := fun _ => rfl
+    symm := fun h => h.symm
+    trans := fun h1 h2 => h1 ▸ h2
   }
 
-#eval ((var₁ "x" + 5) + (9 - 7)) s₀ -- 7
+#eval ((var "x" + 5) + (9 - 7)) s0 -- 7
 
 section Equivalence
 
 -- relational definition is equal to recursive
 private theorem reduce.from_natural
-  (hbig_step: conf ==>ₐ n): conf.1 conf.2 = n :=
+  (hbig_step: conf ==> n): conf.1 conf.2 = n :=
   by induction hbig_step with
-  | addₙ _ _ iha₁ iha₂ => exact iha₁ ▸ iha₂ ▸ rfl
-  | subₙ _ _ iha₁ iha₂ => exact iha₁ ▸ iha₂ ▸ rfl
-  | mulₙ _ _ iha₁ iha₂ => exact iha₁ ▸ iha₂ ▸ rfl
+  | add _ _ iha iha' => exact iha ▸ iha' ▸ rfl
+  | sub _ _ iha iha' => exact iha ▸ iha' ▸ rfl
+  | mul _ _ iha iha' => exact iha ▸ iha' ▸ rfl
   | _ => rfl
 
 private theorem Natural.from_reduce
-  (hred: a s = n): (a, s) ==>ₐ n :=
+  (hred: a s = n): (a, s) ==> n :=
   by induction a generalizing n with
-  | val₁ a => exact hred ▸ big_step.valₙ
-  | var₁ a => exact hred ▸ big_step.varₙ
-  | add₁ a₁ a₂ iha₁ iha₂ =>
-    exact hred ▸ big_step.addₙ (iha₁ rfl) (iha₂ rfl)
-  | sub₁ a₁ a₂ iha₁ iha₂ =>
-    exact hred ▸ big_step.subₙ (iha₁ rfl) (iha₂ rfl)
-  | mul₁ a₁ a₂ iha₁ iha₂ =>
-    exact hred ▸ big_step.mulₙ (iha₁ rfl) (iha₂ rfl)
+  | val a => exact hred ▸ big_step.val
+  | var a => exact hred ▸ big_step.var
+  | add a a' iha iha' =>
+    exact hred ▸ big_step.add (iha rfl) (iha' rfl)
+  | sub a a' iha iha' =>
+    exact hred ▸ big_step.sub (iha rfl) (iha' rfl)
+  | mul a a' iha iha' =>
+    exact hred ▸ big_step.mul (iha rfl) (iha' rfl)
 
 private theorem big_step_eq_reduce:
-  ((a, s) ==>ₐ n) = (a s = n) :=
-  propext ⟨reduce.from_natural, Natural.from_reduce⟩
+  ((a, s) ==> n) = (a s = n) :=
+  propext $ Iff.intro reduce.from_natural Natural.from_reduce
 
 private theorem big_step_eq_reduce':
-  (a, s) ==>ₐ a s :=
+  (a, s) ==> a s :=
   Natural.from_reduce rfl
 
 private theorem big_step_eq_eq_reduce_eq:
-  Natural.big_step.equiv.r a₁ a₂ ↔ reduce.equiv.r a₁ a₂ := by
+  Natural.big_step.equiv.r a a' <-> reduce.equiv.r a a' := by
   simp only [Setoid.r, eq_iff_iff]
   constructor
   . intro h s
-    specialize @h s (a₂ s)
+    specialize @h s (a' s)
     rw [big_step_eq_reduce, big_step_eq_reduce, eq_self, iff_true] at h
     exact h
   . intro h s _
