Semantics/Imp/Lang.lean
@@ -1,68 +1,68 @@
 import Semantics.Maps
 
 def State := Map Int
-def s₀: State := Map.default 0
+def s0: State := Map.default 0
 
-#eval s₀ "x"
-#eval (s₀["x" ← 3]["x" ← 4]) "x"
-#eval (s₀["x" ← 3]["x" ← 4]["x" ← 7]) "x" -- 7
+#eval s0 "x"
+#eval (s0["x" <- 3]["x" <- 4]) "x"
+#eval (s0["x" <- 3]["x" <- 4]["x" <- 7]) "x" -- 7
 
-example: s₀["x" ← 3] = s₀["x" ← 4]["x" ← 3] := Map.eval_last.symm
+example: s0["x" <- 3] = s0["x" <- 4]["x" <- 3] := Map.forget.symm
 
 inductive Aexp where
-  | val₁ : Int → Aexp
-  | var₁ : String → Aexp
+  | val : Int -> Aexp
+  | var : String -> Aexp
   -- arithmetic
-  | add₁ : Aexp → Aexp → Aexp
-  | sub₁ : Aexp → Aexp → Aexp
-  | mul₁ : Aexp → Aexp → Aexp
+  | add : Aexp -> Aexp -> Aexp
+  | sub : Aexp -> Aexp -> Aexp
+  | mul : Aexp -> Aexp -> Aexp
 
-instance: OfNat Aexp n := ⟨Aexp.val₁ n⟩
-instance: Add Aexp := ⟨Aexp.add₁⟩
-instance: Sub Aexp := ⟨Aexp.sub₁⟩
-instance: Neg Aexp := ⟨(Aexp.sub₁ 0 ·)⟩
-instance: Mul Aexp := ⟨Aexp.mul₁⟩
+instance: OfNat Aexp n := OfNat.mk $ Aexp.val n
+instance: Add Aexp := Add.mk Aexp.add
+instance: Sub Aexp := Sub.mk Aexp.sub
+instance: Neg Aexp := Neg.mk (Aexp.sub 0 .)
+instance: Mul Aexp := Mul.mk Aexp.mul
 
 -- x + 3
-#check Aexp.var₁ "x" + 3
+#check Aexp.var "x" + 3
 
 -- x * -3
-#check Aexp.var₁ "x" * -3
+#check Aexp.var "x" * -3
 
 inductive Bexp where
   -- constants
-  | true₁
-  | false₁
+  | true
+  | false
   -- boolean
-  | not₁ : Bexp → Bexp
-  | and₁ : Bexp → Bexp → Bexp
-  | or₁  : Bexp → Bexp → Bexp
+  | not : Bexp -> Bexp
+  | and : Bexp -> Bexp -> Bexp
+  | or  : Bexp -> Bexp -> Bexp
   -- comparison
-  | eq₁ : Aexp → Aexp → Bexp
-  | le₁ : Aexp → Aexp → Bexp
+  | eq : Aexp -> Aexp -> Bexp
+  | le : Aexp -> Aexp -> Bexp
 
-instance: Complement Bexp := ⟨Bexp.not₁⟩
-instance: AndOp Bexp := ⟨Bexp.and₁⟩
-instance: OrOp Bexp := ⟨Bexp.or₁⟩
+instance: Complement Bexp := Complement.mk Bexp.not
+instance: AndOp Bexp := AndOp.mk Bexp.and
+instance: OrOp Bexp := OrOp.mk Bexp.or
 
 -- !(x <= 3)
-#check ~~~(Bexp.le₁ (Aexp.var₁ "x") 3)
+#check ~~~(Bexp.le (Aexp.var "x") 3)
 
 inductive Com where
-  | skip₁
-  | cat₁   : Com → Com → Com
-  | ass₁   : String → Aexp → Com
-  | if₁    : Bexp → Com → Com → Com
-  | while₁ : Bexp → Com → Com
+  | skip
+  | cat        : Com -> Com -> Com
+  | ass        : String -> Aexp -> Com
+  | ifelse     : Bexp -> Com -> Com -> Com
+  | whileloop  : Bexp -> Com -> Com
 
-instance: Append Com := ⟨Com.cat₁⟩
+instance: Append Com := Append.mk Com.cat
 
 /-
 ## Syntax
 -/
 -- Meta syntax
-notation "if " c " then " a " else " b " end" => Com.if₁ c a b
-notation "while " c " loop " a " end" => Com.while₁ c a
+notation "if " c " then " a " else " b " end" => Com.ifelse c a b
+notation "while " c " loop " a " end" => Com.whileloop c a
 
 declare_syntax_cat imp
 
@@ -71,15 +71,15 @@ syntax "(" imp ")" : imp
 -- aexp
 syntax num: imp
 syntax ident: imp
-syntax:55 imp:55 "×" imp:56 : imp
+syntax:55 imp:55 "*" imp:56 : imp
 syntax:60 imp:60 "+" imp:61 : imp
 syntax:60 imp:60 "-" imp:61 : imp
 -- bexp
-syntax:65 imp:65 "∧" imp:66 : imp
-syntax:65 imp:65 "∨" imp:66 : imp
+syntax:65 imp:65 "&&" imp:66 : imp
+syntax:65 imp:65 "||" imp:66 : imp
 syntax:70 imp:70 "=" imp:71 : imp
-syntax:70 imp:70 "≤" imp:71 : imp
-syntax:80 "¬" imp:81 : imp
+syntax:70 imp:70 "<=" imp:71 : imp
+syntax:80 "!" imp:81 : imp
 -- com
 syntax:40 imp:40 ";" imp:41 : imp
 syntax:50 imp:50 ":=" imp:51 : imp
@@ -90,36 +90,34 @@ syntax "[|" imp "|]" : term
 
 macro_rules
   -- keywords
-  | `([|skip|]) => `(Com.skip₁)
-  | `([|true|]) => `(Bexp.true₁)
-  | `([|false|]) => `(Bexp.false₁)
+  | `([|skip|]) => `(Com.skip)
+  | `([|true|]) => `(Bexp.true)
+  | `([|false|]) => `(Bexp.false)
   -- general
   | `([|($x)|]) => `([|$x|])
   -- aexp
-  | `([|$x:ident|]) => `(Aexp.var₁ $(Lean.quote (toString x.getId)))
+  | `([|$x:ident|]) => `(Aexp.var $(Lean.quote (toString x.getId)))
   | `([|$n:num|])   => `($n)
   | `([|$x + $y|])  => `([|$x|] + [|$y|])
   | `([|$x - $y|])  => `([|$x|] - [|$y|])
-  | `([|$x × $y|])  => `([|$x|] * [|$y|])
+  | `([|$x * $y|])  => `([|$x|] * [|$y|])
   -- bexp
-  | `([|¬$x|])      => `(~~~[|$x|])
-  | `([|$x ∧ $y|]) => `([|$x|] &&& [|$y|])
-  | `([|$x ∨ $y|]) => `([|$x|] ||| [|$y|])
-  | `([|$x = $y|]) => `(Bexp.eq₁ [|$x|] [|$y|])
-  | `([|$x ≤ $y|]) => `(Bexp.le₁ [|$x|] [|$y|])
+  | `([|!$x|])      => `(~~~[|$x|])
+  | `([|$x && $y|]) => `([|$x|] &&& [|$y|])
+  | `([|$x || $y|]) => `([|$x|] ||| [|$y|])
+  | `([|$x = $y|]) => `(Bexp.eq [|$x|] [|$y|])
+  | `([|$x <= $y|]) => `(Bexp.le [|$x|] [|$y|])
   -- com
-  | `([|$x:ident := $y|]) => `(Com.ass₁ $(Lean.quote (toString x.getId)) [|$y|])
-  | `([|$x ; $y|])       => `(Com.cat₁ [|$x|] [|$y|])
-  | `([|if $b then $x else $y end|]) => `(Com.if₁ [|$b|] [|$x|] [|$y|])
-  | `([|while $b loop $x end|]) => `(Com.while₁ [|$b|] [|$x|])
+  | `([|$x:ident := $y|]) => `(Com.ass $(Lean.quote (toString x.getId)) [|$y|])
+  | `([|$x ; $y|])       => `(Com.cat [|$x|] [|$y|])
+  | `([|if $b then $x else $y end|]) => `(Com.ifelse [|$b|] [|$x|] [|$y|])
+  | `([|while $b loop $x end|]) => `(Com.whileloop [|$b|] [|$x|])
 
 #check [|
 n := 5; i := 2; res := 1;
 
-while i ≤ n loop
-    res := res × i;
+while i <= n loop
+    res := res * i;
     i := i + 1
 end
 |]
-
-def Config := Com × State
