Semantics/Imp/Natural.lean
@@ -3,73 +3,73 @@ import Semantics.Imp.Bexp
 namespace Com
 namespace Natural
 
-inductive big_step: Config → State → Prop
-  | skipₙ:
-    big_step (skip₁, s) s
+inductive big_step: Com × State -> State -> Prop
+  | skip:
+    big_step (skip, s) s
 
-  | assₙ:
-    big_step (ass₁ v a, s) (s[v ← a s])
+  | ass:
+    big_step (ass v a, s) (s[v <- a s])
 
-  | catₙ (s₂: State) (hc₁: big_step (c₁, s₁) s₂) (hc₂: big_step (c₂, s₂) s₃):
-    big_step (c₁++c₂, s₁) s₃
+  | cat (s'': State) (hcatl: big_step (c, s) s'') (hcatr: big_step (c', s'') s'):
+    big_step (c++c', s) s'
 
-  | if₀ₙ (hb: b s₁ = false) (hc₂: big_step (c₂, s₁) s₂):
-    big_step (if b then c₁ else c₂ end, s₁) s₂
+  | iffalse (hcond: b s = false) (hifright: big_step (c', s) s'):
+    big_step (if b then _ else c' end, s) s'
 
-  | if₁ₙ (hb: b s₁ = true) (hc₁: big_step (c₁, s₁) s₂):
-    big_step (if b then c₁ else c₂ end, s₁) s₂
+  | iftrue (hcond: b s) (hifleft: big_step (c, s) s'):
+    big_step (if b then c else _ end, s) s'
 
-  | while₀ₙ (hb: b s₁ = false):
-    big_step (while b loop c end, s₁) s₁
+  | whilefalse (hcond: b s = false):
+    big_step (while b loop c end, s) s
 
-  | while₁ₙ
-    (s₂: State) (hb: b s₁ = true) (hc: big_step (c, s₁) s₂)
-    (hw: big_step (while b loop c end, s₂) s₃):
-    big_step (while b loop c end, s₁) s₃
+  | whiletrue
+    (s'': State) (hcond: b s) (hwhilestep: big_step (c, s) s'')
+    (hwhilerest: big_step (while b loop c end, s'') s'):
+    big_step (while b loop c end, s) s'
 
-infix:10 " ==>ₙ " => big_step
+infix:10 " ==> " => big_step
 
-private example:  ([|x := 5|], s₀) ==>ₙ s₀["x" ← 5] := big_step.assₙ
+private example:  ([|x := 5|], s0) ==> s0["x" <- 5] := big_step.ass
 
 private example:
    ([|
       x := 2;
-      if x ≤ 1 then
+      if x <= 1 then
         y := 3
       else
         z := 4
       end
-    |], s₀)
-    ==>ₙ s₀["x" ← 2]["z" ← 4] :=
-    big_step.catₙ (s₀["x" ← 2]) big_step.assₙ $ big_step.if₀ₙ rfl big_step.assₙ
+    |], s0)
+    ==> s0["x" <- 2]["z" <- 4] :=
+    big_step.cat (s0["x" <- 2]) big_step.ass $ big_step.iffalse rfl big_step.ass
 
 private example:
-  ([| x := 2; x := 3|], s₀) ==>ₙ s₀["x" ← 3] :=
-  let h1: s₀["x" ← 3] = s₀["x" ← 2]["x" ← 3] :=
-    Map.eval_last.symm
-  h1 ▸ big_step.catₙ _ big_step.assₙ big_step.assₙ
+  ([| x := 2; x := 3|], s0) ==> s0["x" <- 3] :=
+  let h1: s0["x" <- 3] = s0["x" <- 2]["x" <- 3] :=
+    Map.forget.symm
+  h1 ▸ big_step.cat _ big_step.ass big_step.ass
 
 -- factorial of x = 2
 private example:
   ([|
     x := 2;
     y := 1;
-    while 2 ≤ x loop
-      y := y × x;
+    while 2 <= x loop
+      y := y * x;
       x := x - 1
     end
-  |], s₀)
-  ==>ₙ s₀["x" ← 2]["y" ← 1]["y" ← 2]["x" ← 1] := by
-  apply big_step.catₙ (s₀["x" ← 2]["y" ← 1])
-  apply big_step.catₙ (s₀["x" ← 2])
-  apply big_step.assₙ
-  apply big_step.assₙ
-  apply big_step.while₁ₙ (s₀["x" ← 2]["y" ← 1]["y" ← 2]["x" ← 1])
+  |], s0)
+  ==> s0["x" <- 2]["y" <- 1]["y" <- 2]["x" <- 1] := by
+  apply big_step.cat (s0["x" <- 2]["y" <- 1])
+  apply big_step.cat (s0["x" <- 2])
+  apply big_step.ass
+  apply big_step.ass
+  apply big_step.whiletrue (s0["x" <- 2]["y" <- 1]["y" <- 2]["x" <- 1])
   apply rfl
-  apply big_step.catₙ (s₀["x" ← 2]["y" ← 1]["y" ← 2])
-  apply big_step.assₙ
-  apply big_step.assₙ
-  apply big_step.while₀ₙ
+  apply big_step.cat (s0["x" <- 2]["y" <- 1]["y" <- 2])
+  apply big_step.ass
+  apply big_step.ass
+  apply big_step.whilefalse
   apply rfl
 
 /-
@@ -77,54 +77,57 @@ private example:
 -/
 
 theorem skip_eq:
-  ((skip₁, s₁) ==>ₙ s₂) = (s₁ = s₂) :=
+  ((skip, s) ==> s') = (s = s') :=
   propext {
-    mp := λ (big_step.skipₙ) ↦ rfl,
-    mpr := (· ▸ big_step.skipₙ)
+    mp := fun (big_step.skip) => rfl,
+    mpr := (· ▸ big_step.skip)
   }
 
 theorem cat_eq:
-  ((c₁++c₂, s₁) ==>ₙ s₃) = ∃s₂, ((c₁, s₁) ==>ₙ s₂) ∧ ((c₂, s₂) ==>ₙ s₃) :=
+  ((c++c', s) ==> s') = ∃s'', ((c, s) ==> s'') ∧ ((c', s'') ==> s') :=
   propext {
-    mp := λ (big_step.catₙ s₂ h₁ h₂) ↦ ⟨s₂, h₁, h₂⟩,
-    mpr := λ ⟨s₂, h₁, h₂⟩ ↦ big_step.catₙ s₂ h₁ h₂
+    mp := fun (big_step.cat s'' hcatl hcatr) => Exists.intro s'' $ And.intro hcatl hcatr,
+    mpr := fun (Exists.intro s'' $ And.intro hcatl hcatr) => big_step.cat s'' hcatl hcatr
   }
 
 theorem if_eq:
-  ((if b then c₁ else c₂ end, s₁) ==>ₙ s₂)
-    = bif b s₁ then (c₁, s₁) ==>ₙ s₂ else (c₂, s₁) ==>ₙ s₂ :=
+  ((if b then c else c' end, s) ==> s')
+    = bif b s then (c, s) ==> s' else (c', s) ==> s' :=
   propext {
-    mp := λ hmp ↦ match hmp with
-      | big_step.if₁ₙ hb h | big_step.if₀ₙ hb h => hb ▸ h,
-    mpr := match hb: b s₁ with
-      | true => (big_step.if₁ₙ hb ·)
-      | false => (big_step.if₀ₙ hb ·)
+    mp := fun hmp => match hmp with
+      | big_step.iftrue hb h | big_step.iffalse hb h => hb ▸ h,
+    mpr := match hb: b s with
+      | true => (big_step.iftrue hb .)
+      | false => (big_step.iffalse hb .)
   }
 
 theorem if_eq':
-  ((if b then c₁ else c₂ end, s₁) ==>ₙ s₂)
-    = ((bif b s₁ then c₁ else c₂, s₁) ==>ₙ s₂) :=
+  ((if b then c else c' end, s) ==> s')
+    = ((bif b s then c else c', s) ==> s') :=
   propext {
-    mp := λ hmp ↦ match hmp with
-      | big_step.if₁ₙ hb h | big_step.if₀ₙ hb h => hb ▸ h,
-    mpr := match hb: b s₁ with
-      | true => (big_step.if₁ₙ hb ·)
-      | false => (big_step.if₀ₙ hb ·)
+    mp := fun hmp => match hmp with
+      | big_step.iftrue hcond hif | big_step.iffalse hcond hif =>
+        hcond ▸ hif,
+    mpr := match hcond: b s with
+      | true => (big_step.iftrue hcond .)
+      | false => (big_step.iffalse hcond .)
   }
 
 theorem while_eq:
-  ((while b loop c end, s₁) ==>ₙ s₃) =
-    bif b s₁ then
-      ∃s₂, ((c, s₁) ==>ₙ s₂) ∧ ((while b loop c end, s₂) ==>ₙ s₃)
+  ((while b loop c end, s) ==> s') =
+    bif b s then
+      ∃s'', ((c, s) ==> s'') ∧ ((while b loop c end, s'') ==> s')
     else
-      s₁ = s₃ :=
+      s = s' :=
   propext {
-    mp := λ hmp ↦ match hmp with
-      | big_step.while₁ₙ s₂ hb hc hw => hb ▸ ⟨s₂, hc, hw⟩
-      | big_step.while₀ₙ hb => hb ▸ rfl,
-    mpr := match hb: b s₁ with
-      | true => λ ⟨s₂, h₁, h₂⟩ ↦ big_step.while₁ₙ s₂ hb h₁ h₂
-      | false => (· ▸ big_step.while₀ₙ hb)
+    mp := fun hmp => match hmp with
+      | big_step.whiletrue s'' hcond hwhilestep hwhilerest =>
+        hcond ▸ (Exists.intro s'' $ And.intro hwhilestep hwhilerest)
+      | big_step.whilefalse hb => hb ▸ rfl,
+    mpr := match hb: b s with
+      | true => fun (Exists.intro s'' $ And.intro hwhilestep hwhilerest) =>
+        big_step.whiletrue s'' hb hwhilestep hwhilerest
+      | false => (. ▸ big_step.whilefalse hb)
   }
 
 /-
@@ -132,70 +135,66 @@ theorem while_eq:
 -/
 
 instance equiv: Setoid Com where
-  r c₁ c₂ := ∀{s₁ s₂: State}, ((c₁, s₁) ==>ₙ s₂) ↔ ((c₂, s₁) ==>ₙ s₂)
+  r c c' := ∀{s s': State}, ((c, s) ==> s') <-> ((c', s) ==> s')
   iseqv := {
-    refl := λ _ ↦ Iff.rfl
-    symm := (·.symm)
-    trans := λ h1 h2 ↦ h1.trans h2
+    refl := fun _ => Iff.rfl
+    symm := (Iff.symm .)
+    trans := fun h1 h2 => h1.trans h2
   }
 
-theorem skipl:
-  (skip₁++c) ≈ c :=
-  {
-    mp := λ (big_step.catₙ _ hc hd) ↦ skip_eq.mp hc ▸ hd,
-    mpr := (big_step.catₙ _ big_step.skipₙ ·)
+theorem skipl: (skip++c) ≈ c := {
+    mp := fun (big_step.cat _ hcatl hcatr) => skip_eq.mp hcatl ▸ hcatr,
+    mpr := (big_step.cat _ big_step.skip .)
   }
 
-theorem skipr:
-  (c++skip₁) ≈ c :=
-  {
-    mp := λ (big_step.catₙ _ hc hd) ↦ skip_eq.mp hd ▸ hc,
-    mpr := (big_step.catₙ _ · big_step.skipₙ)
+theorem skipr: (c++skip) ≈ c := {
+    mp := fun (big_step.cat _ hc hd) => skip_eq.mp hd ▸ hc,
+    mpr := (big_step.cat _ · big_step.skip)
   }
 
-theorem cond_true (hb: b ≈ Bexp.true₁):
-  if b then c₁ else c₂ end ≈ c₁ := by
+theorem cond_true (hb: b ≈ Bexp.true):
+  if b then c else c' end ≈ c := by
   intro _ _
   rw [if_eq, hb]
   rfl
 
-theorem cond_false (hb: b ≈ Bexp.false₁):
-  if b then c₁ else c₂ end ≈ c₂ := by
+theorem cond_false (hb: b ≈ Bexp.false):
+  if b then c else c' end ≈ c' := by
   intro _ _
   rw [if_eq, hb]
   rfl
 
 theorem loop_unfold:
   while b loop c end ≈
-    if b then c++while b loop c end else skip₁ end := by
-  intro s₁ s₃
+    if b then c++while b loop c end else skip end := by
+  intro s _s''
   rw [if_eq']
   constructor
   . intro hmp
     match hmp with
-    | big_step.while₁ₙ s₂ hb hc hw => exact hb ▸ big_step.catₙ s₂ hc hw
-    | big_step.while₀ₙ hb => exact hb ▸ big_step.skipₙ
-  . match hb: b s₁ with
+    | big_step.whiletrue s' hb hc hw => exact hb ▸ big_step.cat s' hc hw
+    | big_step.whilefalse hb => exact hb ▸ big_step.skip
+  . match hb: b s with
     | false =>
-      intro (big_step.skipₙ)
-      exact big_step.while₀ₙ hb
+      intro (big_step.skip)
+      exact big_step.whilefalse hb
     | true =>
-      intro (big_step.catₙ s₂ hc hw)
-      exact big_step.while₁ₙ s₂ hb hc hw
+      intro (big_step.cat s' hc hw)
+      exact big_step.whiletrue s' hb hc hw
 
 /-
 ## Non termination
 -/
 
-theorem loop_tt (htrue: b ≈ Bexp.true₁):
-  ¬((while b loop c end, s) ==>ₙ t) := by
+theorem loop_tt (htrue: b ≈ Bexp.true):
+  Not ((while b loop c end, s) ==> s') := by
   intro hmp
   generalize hconf: (while b loop c end, s) = conf at hmp
   induction hmp generalizing s with
-  | while₁ₙ _ _ _ _ _ ihw =>
+  | whiletrue _ _ _ _ _ ihw =>
     match hconf with
     | Eq.refl _ => exact ihw rfl
-  | while₀ₙ hb =>
+  | whilefalse hb =>
     match hconf with
     | Eq.refl _ =>
       rw [htrue] at hb
@@ -208,42 +207,42 @@ theorem loop_tt (htrue: b ≈ Bexp.true₁):
 ## Determinism
 -/
 
-theorem deterministic
-  (hps₁: conf ==>ₙ s₁) (hps₂: conf ==>ₙ s₂): s₁ = s₂ :=
-  by induction hps₁ generalizing s₂ with
-  | skipₙ => match hps₂ with | big_step.skipₙ => rfl
-  | assₙ => match hps₂ with | big_step.assₙ => rfl
-  | catₙ _ _ _ ihc₁ ihc₂ =>
-    match hps₂ with
-    | big_step.catₙ _ hc₁ hc₂ =>
-      exact ihc₂ (ihc₁ hc₁ ▸ hc₂)
-  | if₁ₙ hb _ ihc₁ =>
-    match hps₂ with
-    | big_step.if₁ₙ _ hc₁ =>
-      exact ihc₁ hc₁
-    | big_step.if₀ₙ hb₁ _ =>
+theorem deterministic {conf: Com × State}
+  (hps: conf ==> s) (hps': conf ==> s'): s = s' :=
+  by induction hps generalizing s' with
+  | skip => match hps' with | big_step.skip => rfl
+  | ass => match hps' with | big_step.ass => rfl
+  | cat _ _ _ ihc ihc₂ =>
+    match hps' with
+    | big_step.cat _ hc hc₂ =>
+      exact ihc₂ (ihc hc ▸ hc₂)
+  | iftrue hb _ ihc =>
+    match hps' with
+    | big_step.iftrue _ hc =>
+      exact ihc hc
+    | big_step.iffalse hb₁ _ =>
       rw [hb] at hb₁
       contradiction
-  | if₀ₙ hb _ ihc₂ =>
-    match hps₂ with
-    | big_step.if₁ₙ hb₁ _ =>
+  | iffalse hb _ ihc₂ =>
+    match hps' with
+    | big_step.iftrue hb₁ _ =>
       rw [hb] at hb₁
       contradiction
-    | big_step.if₀ₙ _ hd =>
+    | big_step.iffalse _ hd =>
       exact ihc₂ hd
-  | while₁ₙ _ hb _ _ ihc ihw =>
-    match hps₂ with
-    | big_step.while₁ₙ _ _ hc hw =>
+  | whiletrue _ hb _ _ ihc ihw =>
+    match hps' with
+    | big_step.whiletrue _ _ hc hw =>
       exact ihw (ihc hc ▸ hw)
-    | big_step.while₀ₙ hb₁ =>
+    | big_step.whilefalse hb₁ =>
       rw [hb] at hb₁
       contradiction
-  | while₀ₙ hb =>
-    match hps₂ with
-    | big_step.while₁ₙ _ hb₁ _ _ =>
+  | whilefalse hb =>
+    match hps' with
+    | big_step.whiletrue _ hb₁ _ _ =>
       rw [hb] at hb₁
       contradiction
-    | big_step.while₀ₙ _ => rfl
+    | big_step.whilefalse _ => rfl
 
 end Natural
 end Com
