Semantics/Imp/Structural.lean
@@ -4,88 +4,90 @@ import Semantics.ReflTransRel
 namespace Com
 namespace Structural
 
-inductive small_step: Config → Config → Prop where
-  | assₛ:
-    small_step (ass₁ v a, s) (skip₁, s[v ← a s])
+inductive small_step: Com × State -> Com × State -> Prop where
+  | ass:
+    small_step (ass v a, s) (skip, s[v <- a s])
 
-  | cat₀ₛ:
-    small_step (skip₁++c, s) (c, s)
+  | skipcat:
+    small_step (skip++c, s) (c, s)
 
-  | catₙₛ (h: small_step (c₁, s₁) (c₂, s₂)):
-    small_step (c₁++c₃, s₁) (c₂++c₃, s₂)
+  | cat (hstep: small_step (c, s) (c', s')):
+    small_step (c++c'', s) (c'++c'', s')
 
-  | ifₛ:
-    small_step (if b then c₁ else c₂ end, s) (bif b s then c₁ else c₂, s)
+  | ifelse:
+    small_step (if b then c else c' end, s) (bif b s then c else c', s)
 
-  | whileₛ:
+  | whileloop:
     small_step (while b loop c end, s)
-          (bif b s then c++while b loop c end else skip₁, s)
+          (bif b s then c++while b loop c end else skip, s)
 
-infixl:10 " =>ₛ " => small_step
+infixl:10 " ~> " => small_step
 
 private example:
-  ([|x := 0; while x ≤ 2 loop x := x + 1 end|], s₀) =>ₛ
-      ([|skip; while x ≤ 2 loop x := x + 1 end|], s₀["x" ← 0]) :=
-  small_step.catₙₛ small_step.assₛ
+  ([|x := 0; while x <= 2 loop x := x + 1 end|], s0) ~>
+      ([|skip; while x <= 2 loop x := x + 1 end|], s0["x" <- 0]) :=
+  small_step.cat small_step.ass
 
 theorem cat_eq:
-  ((c₁++c₃, s₁) =>ₛ conf)
-    = ((∃c₂ s₂, ((c₁, s₁) =>ₛ (c₂, s₂)) ∧ conf = (c₂++c₃, s₂))
-      ∨ (c₁ = skip₁ ∧ conf = (c₃, s₁))) :=
+  ((c++c'', s) ~> conf)
+    = ((∃c' s', ((c, s) ~> (c', s')) ∧ conf = (c'++c'', s'))
+      ∨ (c = skip ∧ conf = (c'', s))) :=
   propext {
-    mp := λ hmp ↦ match hmp with
-      | small_step.cat₀ₛ => Or.inr ⟨rfl, rfl⟩
-      | small_step.catₙₛ h => Or.inl ⟨_, _, h, rfl⟩,
-    mpr := λ hmpr ↦ match hmpr with
-      | Or.inl ⟨_c₂, _s₂, h₁, h₂⟩ => h₂ ▸ small_step.catₙₛ h₁
-      | Or.inr ⟨h₁, h₂⟩ => h₁ ▸ h₂ ▸ small_step.cat₀ₛ
+    mp := fun hmp => match hmp with
+      | small_step.skipcat => Or.inr $ And.intro rfl rfl
+      | small_step.cat h =>
+        Or.inl $ Exists.intro _ $ Exists.intro _ $ And.intro h rfl,
+    mpr := fun hmpr => match hmpr with
+      | Or.inl (Exists.intro _c' $ Exists.intro _s' $ And.intro hl hr) =>
+        hr ▸ small_step.cat hl
+      | Or.inr (And.intro hl hr) => hl ▸ hr ▸ small_step.skipcat
   }
 
 theorem cond_eq:
-  ((if b then c₁ else c₂ end, s) =>ₛ conf)
-    = (b s ∧ conf = (c₁, s) ∨ b s = false ∧ conf = (c₂, s)) :=
+  ((if b then c else c' end, s) ~> conf)
+    = (b s ∧ conf = (c, s) ∨ b s = false ∧ conf = (c', s)) :=
   propext {
-    mp := λ hmp ↦ match hb: b s with
-      | false => match hmp with | small_step.ifₛ => Or.inr ⟨rfl, hb ▸ rfl⟩
-      | true => match hmp with | small_step.ifₛ => Or.inl ⟨rfl, hb ▸ rfl⟩,
-    mpr := λ hmpr ↦
-      let hss: conf = (bif b s then c₁ else c₂, s) :=
+    mp := fun hmp => match hb: b s with
+      | false => match hmp with | small_step.ifelse => Or.inr $ And.intro rfl $ hb ▸ rfl
+      | true => match hmp with | small_step.ifelse => Or.inl $ And.intro rfl $ hb ▸ rfl,
+    mpr := fun hmpr =>
+      let hss: conf = (bif b s then c else c', s) :=
         match hb: b s with
-        | true => match hb ▸ hmpr with | Or.inl ⟨_, h₂⟩ => h₂
-        | false => match hb ▸ hmpr with | Or.inr ⟨_, h₂⟩ => h₂
-      hss ▸ small_step.ifₛ
+        | true => match hb ▸ hmpr with | Or.inl (And.intro _ hr) => hr
+        | false => match hb ▸ hmpr with | Or.inr (And.intro _ hr) => hr
+      hss ▸ small_step.ifelse
   }
 
-theorem cond_false (hb: b s₁ = false):
-  ((if b then c₁ else c₂ end, s₁) =>ₛ conf) = (conf = (c₂, s₁)) :=
+theorem cond_false (hb: b s = false):
+  ((if b then c else c' end, s) ~> conf) = (conf = (c', s)) :=
   propext {
-    mp := λ hmp ↦ match hb ▸ cond_eq ▸ hmp with
-      | Or.inr ⟨_, h₂⟩ => h₂,
-    mpr := (cond_eq ▸ Or.inr ⟨hb, ·⟩)
+    mp := fun hmp => match hb ▸ cond_eq ▸ hmp with
+      | Or.inr (And.intro _ hr) => hr,
+    mpr := (cond_eq ▸ Or.inr $ And.intro hb .)
   }
 
-infixl:10 " =>ₛ* " => RTL small_step
+infixl:10 " ~>* " => RTL small_step
 
-theorem star.demo₂:
-  ([|x := 2; while 0 ≤ x loop x := x + 1 end|], s₀) =>ₛ*
-      ([|while 0 ≤ x loop x := x + 1 end|], s₀["x" ← 2]) :=
-  RTL.head (small_step.catₙₛ small_step.assₛ) (RTL.head small_step.cat₀ₛ RTL.refl)
+theorem star.demo':
+  ([|x := 2; while 0 <= x loop x := x + 1 end|], s0) ~>*
+      ([|while 0 <= x loop x := x + 1 end|], s0["x" <- 2]) :=
+  RTL.head (small_step.cat small_step.ass) (RTL.head small_step.skipcat RTL.refl)
 
 theorem star.cat_skip_cat
-  (hc₁: (c₁, s₁) =>ₛ* (skip₁, s₂)):
-  (c₁++c₂, s₁) =>ₛ* (skip₁++c₂, s₂) :=
-  RTL.lift (λ (c₁, s) ↦ (c₁++c₂, s)) (λ h ↦ small_step.catₙₛ h) hc₁
+  (hc: (c, s) ~>* (skip, s')):
+  (c++c', s) ~>* (skip++c', s') :=
+  RTL.lift (fun (c, s) => (c++c', s)) (fun h => small_step.cat h) hc
 
 theorem star.cat
-  (hc₁: (c₁, s₁) =>ₛ* (skip₁, s₂))
-  (hc₂: (c₂, s₂) =>ₛ* (skip₁, s₃)):
-  (c₁++c₂, s₁) =>ₛ* (skip₁, s₃) :=
-  RTL.trans (cat_skip_cat hc₁) (RTL.trans (RTL.single small_step.cat₀ₛ) hc₂)
+  (hc: (c, s) ~>* (skip, s'))
+  (hc': (c', s') ~>* (skip, s'')):
+  (c++c', s) ~>* (skip, s'') :=
+  RTL.trans (cat_skip_cat hc) (RTL.trans (RTL.single small_step.skipcat) hc')
 
 theorem star.cat_no_influence
-  (hc₁: (c₁, s) =>ₛ* (skip₁, s₁)):
-  (c₁++c₂, s) =>ₛ* (c₂, s₁) :=
-  RTL.trans (cat_skip_cat hc₁) (RTL.single small_step.cat₀ₛ)
+  (hc: (c, s) ~>* (skip, s)):
+  (c++c', s) ~>* (c', s) :=
+  RTL.trans (cat_skip_cat hc) (RTL.single small_step.skipcat)
 
 end Structural
 end Com
