Semantics/KnasterTarski.lean
@@ -5,44 +5,45 @@ import Semantics.Set
 
 -- define a partial order
 class PartialOrder (α: Type) extends LE α, LT α where
-  le_refl: ∀a: α, a ≤ a
-  le_trans: ∀⦃a b c: α⦄, a ≤ b → b ≤ c → a ≤ c
-  le_iff_le_not_le: ∀⦃a b: α⦄, a < b ↔ a ≤ b ∧ ¬b ≤ a
-  le_antisymm: ∀⦃a b: α⦄, a ≤ b → b ≤ a → a = b
+  le_refl: ∀a: α, a <= a
+  le_trans: ∀{{a b c: α}}, a <= b -> b <= c -> a <= c
+  le_iff_le_not_le: ∀{{a b: α}}, a < b <-> a <= b ∧ Not (b <= a)
+  le_antisymm: ∀{{a b: α}}, a <= b -> b <= a -> a = b
 
 theorem PartialOrder.le_rfl [PartialOrder α] {a: α}:
-  a ≤ a :=
+  a <= a :=
   le_refl a
 
 theorem Set.le_def (a b : Set α) :
-  a ≤ b ↔ a ⊆ b := Iff.rfl
+  a <= b <-> a ⊆ b := Iff.rfl
 
 instance Set.LT (α: Type): LT (Set α) :=
   {
-    lt := λ a b ↦ a ⊆ b ∧ a ≠ b
+    lt := fun a b => a ⊆ b ∧ a ≠ b
   }
 
 theorem Set.lt_def (a b : Set α):
-  a < b ↔ a ⊆ b ∧ a ≠ b :=
+  a < b <-> a ⊆ b ∧ a ≠ b :=
   Iff.rfl
 
 instance Set.partialOrder: PartialOrder (Set α) :=
   {
-    le := λ a b ↦ a ⊆ b,
-    lt := λ a b ↦ a ⊆ b ∧ a ≠ b,
-    le_refl := λ _ _ ha ↦ ha,
-    le_antisymm := λ _ _ h₁ h₂ ↦ Subset.antisymm h₁ h₂,
-    le_iff_le_not_le := λ _ _ ↦ {
-        mp := λ ⟨h₁, h₂⟩ ↦ ⟨h₁, λ h' ↦ h₂ $ Subset.antisymm h₁ h'⟩
-        mpr := λ ⟨h₁, h₂⟩ ↦ ⟨h₁, λ h' ↦ h₂ $ Subset.from_eq h'.symm⟩
-      }
-    le_trans := λ _ _ _ h₁ h₂ _ ha ↦ h₂ (h₁ ha)
+    le := fun a b => a ⊆ b,
+    lt := fun a b => a ⊆ b ∧ a ≠ b,
+    le_refl := fun _a _b hba => hba,
+    le_antisymm := fun _a _b hab hba => Subset.antisymm hab hba,
+    le_iff_le_not_le := fun _a _b => Iff.intro
+        (fun (And.intro hl hr) =>
+          And.intro hl (fun mp => hr (Subset.antisymm hl mp)))
+        (fun (And.intro hl hr) =>
+          And.intro hl (fun mp => hr (Subset.from_eq (Eq.symm mp))))
+    le_trans := fun _a _b _c hab hbc _x ha => hbc (hab ha)
   }
 
 class CompleteLattice (α: Type) extends PartialOrder α where
-  Inf: Set α → α
-  Inf_le: ∀⦃s: Set α⦄, ∀x ∈ s, Inf s ≤ x
-  le_Inf: ∀⦃s: Set α⦄ ⦃a: α⦄, (∀b ∈ s, a ≤ b) → a ≤ Inf s
+  Inf: Set α -> α
+  Inf_le: ∀{{s: Set α}}, ∀x ∈ s, Inf s <= x
+  le_Inf: ∀{{s: Set α}} {{a: α}}, (∀b ∈ s, a <= b) -> a <= Inf s
 
 theorem inf_unique [CompleteLattice α]
   (s: Set α) (a b: α)
@@ -54,9 +55,9 @@ theorem inf_unique [CompleteLattice α]
 
 instance Set.completeLattice: CompleteLattice (Set α) :=
   {
-    Inf := λ s ↦ {x | ∀ A ∈ s, x ∈ A},
-    Inf_le := λ _ x hx _ ha ↦ ha x hx,
-    le_Inf := λ _ _ h _ hb _ hd ↦ h _ hd hb
+    Inf := fun aa => {x | ∀a ∈ aa, x ∈ a},
+    Inf_le := fun _ x hx _ ha => ha x hx,
+    le_Inf := fun _ _ h _ hb _ hd => h _ hd hb
   }
 
 /-
@@ -66,17 +67,17 @@ instance Set.completeLattice: CompleteLattice (Set α) :=
 namespace Fix
 
 def lfp [CompleteLattice α]
-  (f: α → α): α :=
-  CompleteLattice.Inf {a | f a ≤ a}
+  (f: α -> α): α :=
+  CompleteLattice.Inf {a | f a <= a}
 
-theorem lfp_le [CompleteLattice α] {f: α → α}
-  (h: f a ≤ a):
-  lfp f ≤ a :=
+theorem lfp_le [CompleteLattice α] {f: α -> α}
+  (h: f a <= a):
+  lfp f <= a :=
   CompleteLattice.Inf_le _ h
 
-theorem le_lfp [CompleteLattice α] {f: α → α}
-  (h: ∀a', f a' ≤ a' → a ≤ a'):
-  a ≤ lfp f :=
+theorem le_lfp [CompleteLattice α] {f: α -> α}
+  (h: ∀a', f a' <= a' -> a <= a'):
+  a <= lfp f :=
   CompleteLattice.le_Inf h
 
 end Fix
@@ -86,20 +87,20 @@ end Fix
 -/
 
 def monotone [PartialOrder α] [PartialOrder β]
-  (f: α → β): Prop :=
-  ∀a b, a ≤ b → f a ≤ f b
+  (f: α -> β): Prop :=
+  ∀a b, a <= b -> f a <= f b
 
 theorem monotone_id [PartialOrder α]:
-  monotone (@id α) := λ _ _ ↦ id
+  monotone (@id α) := fun _ _ => id
 
 theorem monotone_const [PartialOrder α] [PartialOrder β]
-  (b: β): monotone (λ _: α ↦ b) :=
-  λ _ _ _ ↦ PartialOrder.le_refl b
+  (b: β): monotone (fun _: α => b) :=
+  fun _ _ _ => PartialOrder.le_refl b
 
 theorem monotone_union [PartialOrder α]
-  (f g: α → Set β) (hf: monotone f) (hg: monotone g):
-  monotone (λ a ↦ f a ∪ g a) :=
-  λ a a' ha _b hb ↦
+  (f g: α -> Set β) (hf: monotone f) (hg: monotone g):
+  monotone (fun a => f a ∪ g a) :=
+  fun a a' ha _b hb =>
     match hb with
     | Or.inl h => Or.inl (hf a a' ha h)
     | Or.inr h => Or.inr (hg a a' ha h)
@@ -110,10 +111,10 @@ theorem monotone_union [PartialOrder α]
 
 namespace Fix
 
-theorem lfp_eq [CompleteLattice α] (f: α → α)
+theorem lfp_eq [CompleteLattice α] (f: α -> α)
     (hf: monotone f): lfp f = f (lfp f) :=
-  let h: f (lfp f) ≤ lfp f :=
-    le_lfp (λ a h ↦ PartialOrder.le_trans (hf _ a $ lfp_le h) h)
+  let h: f (lfp f) <= lfp f :=
+    le_lfp (fun a h => PartialOrder.le_trans (hf _ a (lfp_le h)) h)
   PartialOrder.le_antisymm (lfp_le $ hf _ _ h) h
 
 end Fix
