Semantics/Maps.lean
@@ -6,32 +6,32 @@
 ## Total maps
 -/
 
-def Map (α: Type) := String → α
+def Map (α: Type) := String -> α
 
 namespace Map
 
-def default (v: α): Map α := λ _ ↦ v
+def default (v: α): Map α := fun _ => v
 
 def update (m: Map α) (k: String) (v: α) :=
-  λ k' ↦ bif k == k' then v else m k'
+  fun k' => bif k == k' then v else m k'
 
-notation m "[" k " ← " v "]" => Map.update m k v
+notation m "[" k " <- " v "]" => Map.update m k v
 
 theorem eval:
-  (m[k ← v]) k = v := by
+  (m[k <- v]) k = v := by
   unfold Map.update
   rw [beq_self_eq_true, cond_true]
 
-theorem eval_neq (hneq: k != k'):
-  (m[k ← v]) k' = m k' := by
+theorem neval (hneq: k != k'):
+  (m[k <- v]) k' = m k' := by
   unfold Map.update
   rw [bne_iff_ne] at hneq
   rw [Bool.cond_neg]
   rw [beq_eq_false_iff_ne, ne_eq]
   exact hneq
 
-theorem eval_last:
-  m[k ← v₂][k ← v₁] = m[k ← v₁] := by
+theorem forget:
+  m[k <- v'][k <- v] = m[k <- v] := by
   funext k'
   match h: k == k' with
   | true =>
@@ -41,14 +41,14 @@ theorem eval_last:
     unfold Map.update
     rw [h, cond_false, cond_false, cond_false]
 
-theorem eval_swap (hneq : k₁ != k₂):
-  m[k₂ ← v₂][k₁ ← v₁] = m[k₁ ← v₁][k₂ ← v₂] := by
-  funext k'
-  match h: k₁ == k' with
+theorem comm (hneq: k != k'):
+  m[k' <- v'][k <- v] = m[k <- v][k' <- v'] := by
+  funext k''
+  match h: k == k'' with
   | true =>
     unfold Map.update
     rw [h, cond_true]
-    match h': k₂ == k' with
+    match h': k' == k'' with
     | true =>
       rw [eq_of_beq h, eq_of_beq h', bne_iff_ne] at hneq
       contradiction
@@ -58,8 +58,8 @@ theorem eval_swap (hneq : k₁ != k₂):
     unfold Map.update
     rw [h, cond_false, cond_false]
 
-theorem eval_id:
-  m[k ← m k] = m := by
+theorem idem:
+  m[k <- m k] = m := by
   funext k'
   match h: k == k' with
   | true =>
@@ -70,7 +70,7 @@ theorem eval_id:
     rw [h, cond_false]
 
 theorem eval_same:
-  (λ _ ↦ v)[k ← v] = λ _ ↦ v := by
+  (fun _ => v)[k <- v] = fun _ => v := by
   funext k'
   match h: k == k' with
   | true =>
@@ -81,15 +81,15 @@ theorem eval_same:
     rw [h, cond_false]
 
 example (m: Map Nat):
-  m["a" ← 0]["a" ← 2] = m["a" ← 2] := eval_last
+  m["a" <- 0]["a" <- 2] = m["a" <- 2] := forget
 
 example (m: Map Nat):
-  m["a" ← 0]["b" ← 2] = m["b" ← 2]["a" ← 0] := by
-  apply eval_swap
+  m["a" <- 0]["b" <- 2] = m["b" <- 2]["a" <- 0] := by
+  apply comm
   simp only [String.reduceBNe]
 
 example (m: Map Nat):
-  m["a" ← m "a"]["b" ← 0] = m["b" ← 0] := eval_id ▸ rfl
+  m["a" <- m "a"]["b" <- 0] = m["b" <- 0] := idem ▸ rfl
 
 end Map
 
