Semantics/ReflTransRel.lean
@@ -1,35 +1,35 @@
 -- Reflexive transitive relations
-inductive RTL (r : α → α → Prop) (a : α) : α → Prop
-  | refl : RTL r a a
-  | tail : RTL r a b → r b c → RTL r a c
+inductive RTL (r: α -> α -> Prop) (a: α): α -> Prop
+  | refl: RTL r a a
+  | tail: RTL r a b -> r b c -> RTL r a c
 
 namespace RTL
 
-theorem trans (hab : RTL r a b) (hbc : RTL r b c) : RTL r a c := by
+theorem trans (hab: RTL r a b) (hbc: RTL r b c): RTL r a c:= by
   induction hbc with
   | refl => exact hab
   | tail _ hcd hac => exact hac.tail hcd
 
-theorem single (hab : r a b) : RTL r a b :=
+theorem single (hab: r a b): RTL r a b:=
   refl.tail hab
 
-theorem head (hab : r a b) (hbc : RTL r b c) : RTL r a c := by
+theorem head (hab: r a b) (hbc: RTL r b c): RTL r a c:= by
   induction hbc with
   | refl => exact refl.tail hab
   | tail _ hcd hac => exact hac.tail hcd
 
-theorem head_induction_on {P : ∀ a : α, RTL r a b → Prop} {a : α} (h : RTL r a b)
-    (refl : P b refl)
-    (head : ∀{a c} (h' : r a c) (h : RTL r c b), P c h → P a (h.head h')) : P a h := by
+theorem head_induction_on {P: ∀a: α, RTL r a b -> Prop} {a: α} (h: RTL r a b)
+    (refl: P b refl)
+    (head: ∀{a c} (h': r a c) (h: RTL r c b), P c h -> P a (h.head h')): P a h:= by
   induction h with
   | refl => exact refl
   | tail _ hbc ih =>
     apply ih
-    · exact head hbc _ refl
-    · exact λ h1 h2 ↦ head h1 (h2.tail hbc)
+    . exact head hbc _ refl
+    . exact fun h1 h2 => head h1 (h2.tail hbc)
 
-theorem lift {r: α → α → Prop} {p : β → β → Prop} {a b : α} (f : α → β)
-    (h : ∀{a b}, r a b → p (f a) (f b)) (hab : RTL r a b) : RTL p (f a) (f b) := by
+theorem lift {r: α -> α -> Prop} {p: β -> β -> Prop} {a b: α} (f: α -> β)
+    (h: ∀{a b}, r a b -> p (f a) (f b)) (hab: RTL r a b): RTL p (f a) (f b):= by
   induction hab with
   | refl => exact refl
   | tail _ hbc ih => exact ih.tail (h hbc)
